@prefix owl: <http://www.w3.org/2002/07/owl#> .
@prefix xsd: <http://www.w3.org/2001/XMLSchema#> .
@prefix dct: <http://purl.org/dc/terms/> .
@prefix rdf: <http://www.w3.org/1999/02/22-rdf-syntax-ns#> .
@prefix rdfs: <http://www.w3.org/2000/01/rdf-schema#> .
@prefix skos: <http://www.w3.org/2004/02/skos/core#> .
@prefix xl: <http://www.w3.org/2008/05/skos-xl#> .
@prefix org: <http://www.w3.org/ns/org#> .
@prefix foaf: <http://xmlns.com/foaf/0.1/> .
@prefix unvoc: <https://metadata.un.org/schema/> .

# Ontology

unvoc: a owl:Ontology ;
  dct:title "UN Semantic Ontology"@en ;
  dct:description "An ontology for semantic description of various UN resources."@en ;
  
# OWL Classes

unvoc:Thesaurus a rdfs:Class, owl:Class ;
  rdfs:subClassOf skos:ConceptScheme .

unvoc:MemberState a rdfs:Class , owl:Class ;
  rdfs:subClassOf foaf:Agent .

# deprecated as unnecessary; use org:Organization instead
#unvoc:Organization 

# deprecated as unnecessary; use foaf:Person instead
#unvoc:Person 

# This differentiates geographic terms from general subject terms, although a term may be of both classes
unvoc:GeographicTerm a rdfs:Class , owl:Class ;
  rdfs:subClassOf skos:Concept .

# This differentiates place names from general subject terms, although a term may be of both classes  
unvoc:PlaceName a rdfs:Class , owl:Class ;
  rdfs:subClassOf skos:Concept .

# deprecated as unnecessary; use, e.g., org:Role instead
#unvoc:Role 

# Superclass for a voting record
unvoc:VoteRecord a rdfs:Class , owl:Class .
  # voting records have relationships that detail voters and vote characterizations, as well as 
  # document symbols relating to the vote record

# Others: use foaf:Document for document objects; use 
  
# Properties

# DatatypeProperties

# ObjectProperties

#### Voting Records ####

# Proposed predicate. Subject to change.
unvoc:votesNo a rdfs:Property , owl:ObjectProperty ;
  rdfs:comment "Indicates that a Member State cast a No vote on a Vote Record."@en ;
  rdfs:domain unvoc:MemberState ;
  rdfs:range unvoc:VoteRecord ;
  owl:inverseOf unvoc:hasNo .

# Proposed predicate. Subject to change.
unvoc:hasNo a rdfs:Property , owl:ObjectProperty ;
  rdfs:comment "Indicates the list of Member States that voted No on a Vote Record."@en ;
  rdfs:domain unvoc:VoteRecord ;
  rdfs:range unvoc:MemberState ;
  owl:inverseOf unvoc:votesNo

# Proposed predicate. Subject to change.
unvoc:votesYes a rdfs:Property , owl:ObjectProperty ;
  rdfs:comment "Indicates that a Member State cast a Yes vote on a Vote Record."@en ;
  rdfs:domain unvoc:MemberState ;
  rdfs:range unvoc:VoteRecord ;
  owl:inverseOf unvoc:hasYes .

# Proposed predicate. Subject to change.
unvoc:hasYes a rdfs:Property , owl:ObjectProperty ;
  rdfs:comment "Indicates the list of Member States that voted Yes on a Vote Record."@en ;
  rdfs:domain unvoc:VoteRecord ;
  rdfs:range unvoc:MemberState ;
  owl:inverseOf unvoc:votesYes .

# Proposed predicate. Subject to change.
unvoc:abstains a rdfs:Property , owl:ObjectProperty ;
  rdfs:comment "Indicates that a Member State has abstained from voting on a Vote Record."@en ;
  rdfs:domain unvoc:MemberState ;
  rdfs:range unvoc:VoteRecord ;
  owl:inverseOf unvoc:hasAbstention .

# Proposed predicate. Subject to change.
unvoc:hasAbstention a rdfs:Property , owl:ObjectProperty ;
  rdfs:comment "Indicates the list of Member States that abstained from voting on a Vote Record."@en ;
  rdfs:domain unvoc:VoteRecord ;
  rdfs:range unvoc:MemberState ;
  owl:inverseOf unvoc:abstains .

# This predicate is perhaps unnecessary, as it's more important to 
# list the member states that didn't vote than it is to list items 
# they didn't vote on, which can nevertheless be inferred from the 
# next predicate, unvoc:hasNonVoter
#unvoc:??? a rdfs:Property , owl:ObjectProperty ;
#  rdfs:domain unvoc:MemberState ;
#  rdfs:range unvoc:VoteRecord ;
#  owl:inverseOf unvoc:hasNonVoter .

# Proposed predicate. Subject to change.
unvoc:hasNonVoter a rdfs:Property , owl:ObjectProperty ;
  rdfs:comment "Indicates the list of non-voting Member States for a particular Vote Record."@en ;
  rdfs:domain unvoc:VoteRecord ;
  rdfs:range unvoc:MemberState .
  #owl:inverseOf unvoc:noVote .


#### Org and Sessions ####

unvoc:hasSession a rdfs:Property , owl:ObjectProperty ;
  rdfs:comment "Denotes a session belonging to the UN Body."@en ;
  rdfs:domain org:Organization ;
  rdfs:range unvoc:Session ;
  owl:inverseOf unvoc:sessionOf .

unvoc:sessionOf a rdfs:Property , owl:ObjectProperty ;
  rdfs:comment "Denotes a UN Body for which the session was held."@en ;
  rdfs:domain unvoc:Session ;
  rdfs:range org:Organization ;
  owl:inverseOf unvoc:hasSession .
